src/lowparse/pulse/LowParse.Pulse.BitSum.fst
@@ -78,24 +78,11 @@ let jump_bitsum'
     (synth_bitsum'_injective b; synth_bitsum' b)
 
 inline_for_extraction
-```pulse
-fn read_bitsum'_cont
-  (#t: eqtype)
-  (#tot: pos)
-  (#cl: uint_t tot t)
-  (b: bitsum' cl tot)
-  (k_: bitsum'_type b)
-  (pre: vprop)
-  (t': Type0)
-  (post: (t' -> vprop))
-  (phi: (k': bitsum'_type b { k' == k_ }) -> stt t' pre (fun x -> post x))
-  requires pre
-  returns x: t'
-  ensures post x
-{
-  phi k_
-}
-```
+let read_synth_cont_ifthenelse
+  (#t: Type0)
+  (x: Ghost.erased t)
+: Tot (if_combinator_weak (read_synth_cont_t #t x))
+= fun cond iftrue iffalse t' g' -> if cond then iftrue () t' g' else iffalse () t' g'
 
 inline_for_extraction
 let read_bitsum'
@@ -118,40 +105,7 @@ let read_bitsum'
     (synth_bitsum'_recip_inverse b; synth_bitsum'_recip b)
     (
       d
-        stt_cps
-        stt_cps_ifthenelse
-        (read_bitsum'_cont b)
-    )
-
-inline_for_extraction
-let pure_read_synth_cont_ifthenelse
-  (#t: Type0)
-  (x: Ghost.erased t)
-: Tot (if_combinator_weak (pure_read_synth_cont_t #t x))
-= fun cond iftrue iffalse t' g' -> if cond then iftrue () t' g' else iffalse () t' g'
-
-inline_for_extraction
-let pure_read_bitsum'
-  (#t: eqtype)
-  (#tot: pos)
-  (#cl: uint_t tot t)
-  (#b: bitsum' cl tot)
-  (d: destr_bitsum'_t b)
-  (#k: parser_kind)
-  (#p: parser k t)
-  (#s: serializer p)
-  (r: pure_reader s)
-: Tot (pure_reader (tot_serialize_bitsum' b s))
-= pure_read_synth
-    (pure_read_filter
-      r
-      (filter_bitsum' b)
-    )
-    (synth_bitsum'_injective b; synth_bitsum' b)
-    (synth_bitsum'_recip_inverse b; synth_bitsum'_recip b)
-    (
-      d
-        (pure_read_synth_cont_t #(bitsum'_type b))
-        (pure_read_synth_cont_ifthenelse #(bitsum'_type b))
-        (pure_read_synth_cont_init)
+        (read_synth_cont_t #(bitsum'_type b))
+        (read_synth_cont_ifthenelse #(bitsum'_type b))
+        (read_synth_cont_init)
     )
